# baseURI: http://sweetontology.net/sweetAll
# imports: http://sweetontology.net/matr
# imports: http://sweetontology.net/matrAerosol
# imports: http://sweetontology.net/matrElement
# imports: http://sweetontology.net/matrElementalMolecule
# imports: http://sweetontology.net/matrEnergy
# imports: http://sweetontology.net/matrEquipment
# imports: http://sweetontology.net/matrFacility
# imports: http://sweetontology.net/matrIndustrial
# imports: http://sweetontology.net/matrInstrument
# imports: http://sweetontology.net/matrIon
# imports: http://sweetontology.net/matrIsotope
# imports: http://sweetontology.net/matrMineral
# imports: http://sweetontology.net/matrNaturalResource
# imports: http://sweetontology.net/matrOrganicCompound
# imports: http://sweetontology.net/matrParticle
# imports: http://sweetontology.net/matrPlant
# imports: http://sweetontology.net/matrRock
# imports: http://sweetontology.net/matrRockIgneous
# imports: http://sweetontology.net/matrSediment
# imports: http://sweetontology.net/matrWater
# imports: http://sweetontology.net/phen
# imports: http://sweetontology.net/phenAtmo

# imports: http://sweetontology.net/phenAtmoPressure
# imports: http://sweetontology.net/phenAtmoTransport
# imports: http://sweetontology.net/phenAtmoWind
# imports: http://sweetontology.net/phenAtmoWindMesoscale
# imports: http://sweetontology.net/phenBiol
# imports: http://sweetontology.net/phenCryo
# imports: http://sweetontology.net/phenCycle
# imports: http://sweetontology.net/phenCycleMaterial
# imports: http://sweetontology.net/phenEcology
# imports: http://sweetontology.net/phenElecMag
# imports: http://sweetontology.net/phenEnergy
# imports: http://sweetontology.net/phenEnvirImpact
# imports: http://sweetontology.net/phenFluidDynamics
# imports: http://sweetontology.net/phenFluidInstability
# imports: http://sweetontology.net/phenFluidTransport
# imports: http://sweetontology.net/phenGeol
# imports: http://sweetontology.net/phenGeolFault
# imports: http://sweetontology.net/phenGeolGeomorphology
# imports: http://sweetontology.net/phenGeolSeismicity
# imports: http://sweetontology.net/phenGeolTectonic
# imports: http://sweetontology.net/phenGeolVolcano
# imports: http://sweetontology.net/phenHelio
# imports: http://sweetontology.net/phenHydro
# imports: http://sweetontology.net/phenMixing
# imports: http://sweetontology.net/phenOcean
# imports: http://sweetontology.net/phenOceanCoastal
# imports: http://sweetontology.net/phenOceanDynamics
# imports: http://sweetontology.net/phenPlanetClimate
# imports: http://sweetontology.net/phenReaction
# imports: http://sweetontology.net/phenSolid
# imports: http://sweetontology.net/phenStar
# imports: http://sweetontology.net/phenSystem
# imports: http://sweetontology.net/phenSystemComplexity
# imports: http://sweetontology.net/phenWave
# imports: http://sweetontology.net/phenWaveNoise
# imports: http://sweetontology.net/proc
# imports: http://sweetontology.net/procChemical
# imports: http://sweetontology.net/procPhysical
# imports: http://sweetontology.net/procStateChange
# imports: http://sweetontology.net/procWave
# imports: http://sweetontology.net/prop
# imports: http://sweetontology.net/propBinary
# imports: http://sweetontology.net/propCapacity
# imports: http://sweetontology.net/propCategorical
# imports: http://sweetontology.net/propCharge
# imports: http://sweetontology.net/propChemical
# imports: http://sweetontology.net/propConductivity
# imports: http://sweetontology.net/propCount
# imports: http://sweetontology.net/propDifference
# imports: http://sweetontology.net/propDiffusivity
# imports: http://sweetontology.net/propDimensionlessRatio
# imports: http://sweetontology.net/propEnergy
# imports: http://sweetontology.net/propEnergyFlux
# imports: http://sweetontology.net/propFraction
# imports: http://sweetontology.net/propFunction
# imports: http://sweetontology.net/propIndex
# imports: http://sweetontology.net/propMass
# imports: http://sweetontology.net/propMassFlux
# imports: http://sweetontology.net/propOrdinal
# imports: http://sweetontology.net/propPressure
# imports: http://sweetontology.net/propQuantity
# imports: http://sweetontology.net/propRotation
# imports: http://sweetontology.net/propSpace
# imports: http://sweetontology.net/propSpaceDirection
# imports: http://sweetontology.net/propSpaceDistance
# imports: http://sweetontology.net/propSpaceHeight
# imports: http://sweetontology.net/propSpaceLocation
# imports: http://sweetontology.net/propSpaceMultidimensional
# imports: http://sweetontology.net/propSpaceThickness
# imports: http://sweetontology.net/propSpeed
# imports: http://sweetontology.net/propTemperature
# imports: http://sweetontology.net/propTemperatureGradient
# imports: http://sweetontology.net/propTime
# imports: http://sweetontology.net/propTimeFrequency
# imports: http://sweetontology.net/realm
# imports: http://sweetontology.net/realmAstroBody

# imports: http://sweetontology.net/realmAtmo
# imports: http://sweetontology.net/realmAtmoBoundaryLayer
# imports: http://sweetontology.net/realmAtmoWeather
# imports: http://sweetontology.net/realmBiolBiome
# imports: http://sweetontology.net/realmClimateZone
# imports: http://sweetontology.net/realmCryo
# imports: http://sweetontology.net/realmEarthReference
# imports: http://sweetontology.net/realmGeol
# imports: http://sweetontology.net/realmGeolBasin
# imports: http://sweetontology.net/realmGeolConstituent
# imports: http://sweetontology.net/realmGeolContinental
# imports: http://sweetontology.net/realmGeolOrogen
# imports: http://sweetontology.net/realmHydro
# imports: http://sweetontology.net/realmHydroBody
# imports: http://sweetontology.net/realmLandAeolian
# imports: http://sweetontology.net/realmLandCoastal
# imports: http://sweetontology.net/realmLandFluvial
# imports: http://sweetontology.net/realmLandGlacial
# imports: http://sweetontology.net/realmLandOrographic
# imports: http://sweetontology.net/realmLandProtected
# imports: http://sweetontology.net/realmLandTectonic
# imports: http://sweetontology.net/realmLandVolcanic
# imports: http://sweetontology.net/realmLandform
# imports: http://sweetontology.net/realmOcean
# imports: http://sweetontology.net/realmOceanFeature
# imports: http://sweetontology.net/realmOceanFloor
# imports: http://sweetontology.net/realmRegion
# imports: http://sweetontology.net/realmSoil
# imports: http://sweetontology.net/rela
# imports: http://sweetontology.net/relaChemical
# imports: http://sweetontology.net/relaClimate
# imports: http://sweetontology.net/relaHuman
# imports: http://sweetontology.net/relaMath
# imports: http://sweetontology.net/relaPhysical
# imports: http://sweetontology.net/relaProvenance
# imports: http://sweetontology.net/relaSci
# imports: http://sweetontology.net/relaSpace
# imports: http://sweetontology.net/relaTime
# imports: http://sweetontology.net/repr
# imports: http://sweetontology.net/reprDataFormat
# imports: http://sweetontology.net/reprDataModel
# imports: http://sweetontology.net/reprDataProduct
# imports: http://sweetontology.net/reprDataService
# imports: http://sweetontology.net/reprDataServiceAnalysis
# imports: http://sweetontology.net/reprDataServiceGeospatial
# imports: http://sweetontology.net/reprDataServiceReduction
# imports: http://sweetontology.net/reprDataServiceValidation
# imports: http://sweetontology.net/reprMath
# imports: http://sweetontology.net/reprMathFunction
# imports: http://sweetontology.net/reprMathFunctionOrthogonal
# imports: http://sweetontology.net/reprMathGraph
# imports: http://sweetontology.net/reprMathOperation
# imports: http://sweetontology.net/reprMathSolution
# imports: http://sweetontology.net/reprMathStatistics
# imports: http://sweetontology.net/reprSciComponent
# imports: http://sweetontology.net/reprSciFunction
# imports: http://sweetontology.net/reprSciLaw
# imports: http://sweetontology.net/reprSciMethodology
# imports: http://sweetontology.net/reprSciModel
# imports: http://sweetontology.net/reprSciProvenance
# imports: http://sweetontology.net/reprSciUnits
# imports: http://sweetontology.net/reprSpace
# imports: http://sweetontology.net/reprSpaceCoordinate
# imports: http://sweetontology.net/reprSpaceDirection
# imports: http://sweetontology.net/reprSpaceGeometry
# imports: http://sweetontology.net/reprSpaceGeometry3D
# imports: http://sweetontology.net/reprSpaceReferenceSystem
# imports: http://sweetontology.net/reprTime
# imports: http://sweetontology.net/reprTimeDay
# imports: http://sweetontology.net/reprTimeSeason
# imports: http://sweetontology.net/state
# imports: http://sweetontology.net/stateBiological
# imports: http://sweetontology.net/stateChemical
# imports: http://sweetontology.net/stateDataProcessing
# imports: http://sweetontology.net/stateEnergyFlux
# imports: http://sweetontology.net/stateFluid
# imports: http://sweetontology.net/stateOrdinal
# imports: http://sweetontology.net/statePhysical
# imports: http://sweetontology.net/stateRealm
# imports: http://sweetontology.net/stateRole
# imports: http://sweetontology.net/stateRoleBiological
# imports: http://sweetontology.net/stateRoleChemical
# imports: http://sweetontology.net/stateRoleGeographic
# imports: http://sweetontology.net/stateRoleImpact
# imports: http://sweetontology.net/stateRoleRepresentative
# imports: http://sweetontology.net/stateRoleTrust
# imports: http://sweetontology.net/stateSolid
# imports: http://sweetontology.net/stateSpace
# imports: http://sweetontology.net/stateSpaceConfiguration
# imports: http://sweetontology.net/stateSpaceScale
# imports: http://sweetontology.net/stateSpectralBand
# imports: http://sweetontology.net/stateSpectralLine
# imports: http://sweetontology.net/stateStorm
# imports: http://sweetontology.net/stateSystem
# imports: http://sweetontology.net/stateThermodynamic
# imports: http://sweetontology.net/stateTime
# imports: http://sweetontology.net/stateTimeCycle
# imports: http://sweetontology.net/stateTimeFrequency
# imports: http://sweetontology.net/stateTimeGeologic
# imports: http://sweetontology.net/stateVisibility

@prefix : <http://sweetontology.net/sweetAll/> .
@prefix dcterms: <http://purl.org/dc/terms/> .
@prefix owl: <http://www.w3.org/2002/07/owl#> .
@prefix rdf: <http://www.w3.org/1999/02/22-rdf-syntax-ns#> .
@prefix rdfs: <http://www.w3.org/2000/01/rdf-schema#> .
@prefix skos: <http://www.w3.org/2004/02/skos/core#> .
@prefix xsd: <http://www.w3.org/2001/XMLSchema#> .

<http://sweetontology.net/phenGeolTectonic/TectonicAssemblage>
  rdfs:subClassOf :GeologicUnit ;
.
<http://sweetontology.net/realmGeol/DenudationalFeature>
  rdfs:subClassOf :GeomorphicFeature ;
.
<http://sweetontology.net/realmGeol/Depression>
  rdfs:subClassOf :GeomorphicFeature ;
.
<http://sweetontology.net/realmGeol/Dome>
  rdfs:subClassOf :GeomorphicFeature ;
.
<http://sweetontology.net/realmGeol/Embayment>
  rdfs:subClassOf :GeomorphicFeature ;
.
<http://sweetontology.net/realmGeol/Escarpment>
  rdfs:subClassOf :GeomorphicFeature ;
.
<http://sweetontology.net/realmGeol/GeophysicalFeature>
  rdfs:subClassOf :GeologicUnit ;
.
<http://sweetontology.net/realmGeol/InnerCore>
  rdfs:subClassOf [
      a owl:Restriction ;
      owl:allValuesFrom <http://sweetontology.net/realmGeol/Core> ;
      owl:onProperty <http://sweetontology.net/rela/partOf> ;
    ] ;
.
<http://sweetontology.net/realmGeol/LithodemicFeature>
  rdfs:subClassOf :GeologicUnit ;
.
<http://sweetontology.net/realmGeol/OuterCore>
  rdfs:subClassOf [
      a owl:Restriction ;
      owl:allValuesFrom <http://sweetontology.net/realmGeol/Core> ;
      owl:onProperty <http://sweetontology.net/rela/partOf> ;
    ] ;
.
<http://sweetontology.net/realmGeol/Ridge>
  rdfs:subClassOf :GeomorphicFeature ;
.
<http://sweetontology.net/realmGeol/StratigraphicFeature>
  rdfs:subClassOf :GeologicUnit ;
.
<http://sweetontology.net/realmGeolOrogen/RearArc>
  rdfs:subClassOf <http://sweetontology.net/realmGeol/TectonicFeature> ;
.
<http://sweetontology.net/realmGeolOrogen/RetroArc>
  rdfs:subClassOf <http://sweetontology.net/realmGeol/TectonicFeature> ;
.
<http://sweetontology.net/realmHydro/Embankment>
  rdfs:subClassOf :GeomorphicFeature ;
.
<http://sweetontology.net/realmHydro/FloodBank>
  rdfs:subClassOf :GeomorphicFeature ;
.
<http://sweetontology.net/realmHydro/Levee>
  rdfs:subClassOf :GeomorphicFeature ;
.
<http://sweetontology.net/realmHydro/RaisedBank>
  rdfs:subClassOf :GeomorphicFeature ;
.
<http://sweetontology.net/realmHydroBody/Fiord>
  rdfs:subClassOf :GeomorphicFeature ;
.
<http://sweetontology.net/realmLandAeolian/SandDune>
  rdfs:subClassOf :GeomorphicFeature ;
.
<http://sweetontology.net/realmLandCoastal/DeltaBar>
  rdfs:subClassOf :GeomorphicFeature ;
.
<http://sweetontology.net/realmLandTectonic/Diapir>
  rdfs:subClassOf :GeologicUnit ;
.
<http://sweetontology.net/realmLandTectonic/Ophiolite>
  rdfs:subClassOf <http://sweetontology.net/realmGeol/TectonicFeature> ;
.
<http://sweetontology.net/realmLandVolcanic/LavaPlain>
  rdfs:subClassOf :GeomorphicFeature ;
.
<http://sweetontology.net/realmLandform/Landform>
  rdfs:subClassOf :GeomorphicFeature ;
.
<http://sweetontology.net/sweetAll>
  a owl:Ontology ;
  dcterms:license <https://creativecommons.org/publicdomain/zero/1.0/> ;
  rdfs:comment """The semantic web for Earth and environmental terminology (SWEET) is an investigation in improving discovery and use of Earth science data, through software understanding of the semantics of web resources.  SWEET is a collection of ontologies conceptualizing a knowledge space for Earth system science, represented using the web ontology language (OWL). It includes both orthogonal concepts (space, time, Earth realms, physical quantities, etc.) and integrative science knowledge concepts (phenomena, events, etc.).  The ontology is modularized into 224 component files in this version, each representing a different namespace, with numerous dependencies implemented by OWL imports between the namespace.  Component factoring may change in future versions.

The original version was developed by Robert Raskin at JPL (see Raskin and  Pan, 2005: https://doi.org/10.1016/j.cageo.2004.12.004). Stewardship has been taken over by the Earth Science Information Partners Federation (ESIPFed), managed through a GitHub repository at https://github.com/ESIPFed/sweet.  See https://github.com/ESIPFed/sweet/blob/master/CONTRIBUTING.md for information about providing comments or contributing to development of SWEET."""@en ;
  rdfs:label "SWEET Ontology" ;

  owl:imports <http://sweetontology.net/matr> ;


  owl:imports <http://sweetontology.net/matrElement> ;
  owl:imports <http://sweetontology.net/matrElementalMolecule> ;
  owl:imports <http://sweetontology.net/matrEnergy> ;


  owl:imports <http://sweetontology.net/matrIon> ;
  owl:imports <http://sweetontology.net/matrIsotope> ;

  owl:imports <http://sweetontology.net/matrMineral> ;
  owl:imports <http://sweetontology.net/matrNaturalResource> ;
  owl:imports <http://sweetontology.net/matrOrganicCompound> ;
  owl:imports <http://sweetontology.net/matrParticle> ;

  owl:imports <http://sweetontology.net/matrRock> ;
  owl:imports <http://sweetontology.net/matrRockIgneous> ;
  owl:imports <http://sweetontology.net/matrSediment> ;
  owl:imports <http://sweetontology.net/matrWater> ;
  owl:imports <http://sweetontology.net/phen> ;
  owl:imports <http://sweetontology.net/phenAtmo> ;




  owl:imports <http://sweetontology.net/phenCryo> ;
  owl:imports <http://sweetontology.net/phenCycle> ;
  owl:imports <http://sweetontology.net/phenCycleMaterial> ;
  owl:imports <http://sweetontology.net/phenEcology> ;

  owl:imports <http://sweetontology.net/phenEnergy> ;


  owl:imports <http://sweetontology.net/phenGeol> ;
  owl:imports <http://sweetontology.net/phenGeolFault> ;
  owl:imports <http://sweetontology.net/phenGeolGeomorphology> ;
  owl:imports <http://sweetontology.net/phenGeolSeismicity> ;
  owl:imports <http://sweetontology.net/phenGeolTectonic> ;
  owl:imports <http://sweetontology.net/phenGeolVolcano> ;

  owl:imports <http://sweetontology.net/phenHydro> ;
  owl:imports <http://sweetontology.net/phenMixing> ;
  owl:imports <http://sweetontology.net/phenOcean> ;
  owl:imports <http://sweetontology.net/phenOceanCoastal> ;

  owl:imports <http://sweetontology.net/phenPlanetClimate> ;

  owl:imports <http://sweetontology.net/phenSolid> ;

  owl:imports <http://sweetontology.net/phenSystem> ;


  owl:imports <http://sweetontology.net/proc> ;
  owl:imports <http://sweetontology.net/procChemical> ;
  owl:imports <http://sweetontology.net/procPhysical> ;

  owl:imports <http://sweetontology.net/prop> ;
  owl:imports <http://sweetontology.net/propBinary> ;

  owl:imports <http://sweetontology.net/propCategorical> ;

  owl:imports <http://sweetontology.net/propChemical> ;

  owl:imports <http://sweetontology.net/propCount> ;
  owl:imports <http://sweetontology.net/propDifference> ;

  owl:imports <http://sweetontology.net/propDimensionlessRatio> ;
  owl:imports <http://sweetontology.net/propEnergy> ;
  owl:imports <http://sweetontology.net/propEnergyFlux> ;
  owl:imports <http://sweetontology.net/propFraction> ;
  owl:imports <http://sweetontology.net/propFunction> ;

  owl:imports <http://sweetontology.net/propMass> ;
  owl:imports <http://sweetontology.net/propMassFlux> ;
  owl:imports <http://sweetontology.net/propOrdinal> ;
  owl:imports <http://sweetontology.net/propPressure> ;
  owl:imports <http://sweetontology.net/propQuantity> ;

  owl:imports <http://sweetontology.net/propSpace> ;

  owl:imports <http://sweetontology.net/propSpeed> ;
  owl:imports <http://sweetontology.net/propTemperature> ;

  owl:imports <http://sweetontology.net/propTime> ;
  owl:imports <http://sweetontology.net/propTimeFrequency> ;
  owl:imports <http://sweetontology.net/realm> ;


  owl:imports <http://sweetontology.net/realmAtmo> ;



  owl:imports <http://sweetontology.net/realmClimateZone> ;
  owl:imports <http://sweetontology.net/realmCryo> ;
  owl:imports <http://sweetontology.net/realmEarthReference> ;
  owl:imports <http://sweetontology.net/realmGeol> ;
  owl:imports <http://sweetontology.net/realmGeolBasin> ;
  owl:imports <http://sweetontology.net/realmGeolConstituent> ;
  owl:imports <http://sweetontology.net/realmGeolContinental> ;
  owl:imports <http://sweetontology.net/realmGeolOrogen> ;
  owl:imports <http://sweetontology.net/realmHydro> ;
  owl:imports <http://sweetontology.net/realmHydroBody> ;
  owl:imports <http://sweetontology.net/realmLandAeolian> ;
  owl:imports <http://sweetontology.net/realmLandCoastal> ;
  owl:imports <http://sweetontology.net/realmLandFluvial> ;
  owl:imports <http://sweetontology.net/realmLandGlacial> ;
  owl:imports <http://sweetontology.net/realmLandOrographic> ;
  owl:imports <http://sweetontology.net/realmLandProtected> ;
  owl:imports <http://sweetontology.net/realmLandTectonic> ;
  owl:imports <http://sweetontology.net/realmLandVolcanic> ;
  owl:imports <http://sweetontology.net/realmLandform> ;
  owl:imports <http://sweetontology.net/realmOcean> ;
  owl:imports <http://sweetontology.net/realmOceanFeature> ;
  owl:imports <http://sweetontology.net/realmOceanFloor> ;
  owl:imports <http://sweetontology.net/realmRegion> ;
  owl:imports <http://sweetontology.net/realmSoil> ;
  owl:imports <http://sweetontology.net/rela> ;
  owl:imports <http://sweetontology.net/relaChemical> ;
  owl:imports <http://sweetontology.net/relaClimate> ;


  owl:imports <http://sweetontology.net/relaPhysical> ;
  owl:imports <http://sweetontology.net/relaProvenance> ;
  owl:imports <http://sweetontology.net/relaSci> ;
  owl:imports <http://sweetontology.net/relaSpace> ;
  owl:imports <http://sweetontology.net/relaTime> ;
  owl:imports <http://sweetontology.net/repr> ;

  owl:imports <http://sweetontology.net/reprMath> ;


  owl:imports <http://sweetontology.net/reprSciUnits> ;
  owl:imports <http://sweetontology.net/reprSpace> ;

  owl:imports <http://sweetontology.net/reprTime> ;
  owl:imports <http://sweetontology.net/reprTimeDay> ;
  owl:imports <http://sweetontology.net/reprTimeSeason> ;
  owl:imports <http://sweetontology.net/state> ;

  owl:imports <http://sweetontology.net/stateChemical> ;

  owl:imports <http://sweetontology.net/stateEnergyFlux> ;
  owl:imports <http://sweetontology.net/stateFluid> ;
  owl:imports <http://sweetontology.net/stateOrdinal> ;
  owl:imports <http://sweetontology.net/statePhysical> ;
  owl:imports <http://sweetontology.net/stateRealm> ;
  owl:imports <http://sweetontology.net/stateRole> ;



  owl:imports <http://sweetontology.net/stateSolid> ;
  owl:imports <http://sweetontology.net/stateSpace> ;


  owl:imports <http://sweetontology.net/stateSystem> ;
  owl:imports <http://sweetontology.net/stateThermodynamic> ;
  owl:imports <http://sweetontology.net/stateTime> ;
  owl:imports <http://sweetontology.net/stateTimeCycle> ;
  owl:imports <http://sweetontology.net/stateTimeFrequency> ;
  owl:imports <http://sweetontology.net/stateTimeGeologic> ;
  owl:imports <http://sweetontology.net/stateVisibility> ;
  owl:versionInfo "3.5.0" ;
.
:GeologicUnit
  a owl:Class ;
  rdfs:comment "a body of material in the Earth whose complete and precise extent is inferred to exist (NADM GeologicUnit, Stratigraphic unit in sense of NACSN or International Stratigraphic Code), or a classifier used to characterize parts of the Earth (e.g. lithologic map unit like 'granitic rock' or 'alluvial deposit', surficial units like 'till' or 'old alluvium'). GeoSciML v3.2" ;
  rdfs:label "Geologic Unit "@en ;
  rdfs:subClassOf <http://sweetontology.net/realmGeol/GeologicFeature> ;
  skos:prefLabel "Geologic Unit "@en ;
.
:GeomorphicFeature
  a owl:Class ;
  rdfs:comment "A feature describing the shape and nature of the Earth's land surface (ie, a landform).  These landforms may be created by natural Earth processes (eg, river channel, beach, moraine, mountain) or through human (anthropogenic) activity (eg, dredged channel, reclaimed land, mine waste dumps). GeoSciML v3.2" ;
  rdfs:label "Geomorphic Feature "@en ;
  rdfs:subClassOf <http://sweetontology.net/realmGeol/GeologicFeature> ;
  skos:prefLabel "Geomorphic Feature  "@en ;
.
